src/coq/optimisations/SANDBOX/FindSearch.v
@@ -1,0 +1,17 @@
+(* Consider the following structure: *)
+
+Definition iid := nat.
+Definition data := nat.
+
+Definition bid := nat.
+Definition fid := nat.
+
+Definition listA := list (bid * data).
+Definition listB := list (fid * listA).
+
+
+Fixpoint searchListA (b:bid) (l:listA) : option (bid * data) :=
+match l with
+  | nil => None
+  | (_::_)%list => None
+end.
