src/coq/optimisations/add_instrproof.v
@@ -1,12 +1,19 @@
 
 Require Import ZArith List String Omega.
-Require Import  Vellvm.Ollvm_ast Vellvm.Classes Vellvm.Util Vellvm.optimisations.transform.
+Require Import  Vellvm.Ollvm_ast Vellvm.Classes Vellvm.Util Vellvm.CFGProp Vellvm.CFG.
+
+Require Import Vellvm.optimisations.transform.
+Require Import Vellvm.optimisations.add_instr.
 Require Import paco.
 Require Import Vellvm.Memory.
 Require Import Vellvm.Effects.
-Require Import Vellvm.optimisations.add_instr.
 
 
+Print find_function.
+
+
+
+(*Let's prove the find_function does not get impacted by both*)
 
 
 Definition unroll (t:Trace ()) :=
@@ -15,73 +22,95 @@ match t with
   | Tau a b => Tau a b
 end.
 
+(*Let's recap:
+This optimisation adds a useless instruction to a block if the terminator is a return void
 
+
+Informally reasoning, there are two possible cases:
+  -The terminator instruction is a return void. This means that the state doesn't matter because it doesn't impact the terminator instruction.
+  -The terminator is not a return void. The instruction does not get added meaning the execution doesn't get affected.
+
+
+
+Essentially, we want to solve this by induction on the terminator instruction of a block.
+
+
+*)
+
+
+
+Print prog_optimise.
+Print optimise.
 Lemma do_nothing_correct : forall mem st prog, trace_equiv (memD mem (sem prog st)) (memD mem (sem (prog_optimise prog) st)).
 Proof. pcofix CIH.
 intros.
 pfold.
 
+(*unroll right*)
+assert ((memD mem (sem prog st)) = unroll (memD mem (sem prog st)) ).
+destruct (memD mem (sem prog st)) ; eauto.
+rewrite H. clear H.
 
-assert ((memD mem (sem prog st)) = unroll (memD mem (sem prog st))).
-destruct (memD mem (sem prog st)); eauto.
-induction prog. induction m_definitions.
--(*empty*) admit.
--(*mdefinitions*)destruct a. destruct df_instrs. destruct blks. 
-  +assert ((memD mem
-     (sem
-        {|
-        m_name := m_name;
-        m_target := m_target;
-        m_datalayout := m_datalayout;
-        m_globals := m_globals;
-        m_declarations := m_declarations;
-        m_definitions := {|
-                         df_prototype := df_prototype;
-                         df_args := df_args;
-                         df_instrs := {|
-                                      CFG.init := init;
-                                      CFG.blks := [];
-                                      CFG.glbl := glbl |} |} :: m_definitions |}
-        st)) = unroll (memD mem
-     (sem
-        {|
-        m_name := m_name;
-        m_target := m_target;
-        m_datalayout := m_datalayout;
-        m_globals := m_globals;
-        m_declarations := m_declarations;
-        m_definitions := {|
-                         df_prototype := df_prototype;
-                         df_args := df_args;
-                         df_instrs := {|
-                                      CFG.init := init;
-                                      CFG.blks := [];
-                                      CFG.glbl := glbl |} |} :: m_definitions |}
-        st))). destruct (memD mem
-     (sem
-        {|
-        m_name := m_name;
-        m_target := m_target;
-        m_datalayout := m_datalayout;
-        m_globals := m_globals;
-        m_declarations := m_declarations;
-        m_definitions := {|
-                         df_prototype := df_prototype;
-                         df_args := df_args;
-                         df_instrs := {|
-                                      CFG.init := init;
-                                      CFG.blks := [];
-                                      CFG.glbl := glbl |} |} :: m_definitions |}
-        st)); eauto.
+(*unroll left*)
+assert ((memD mem (sem (prog_optimise prog) st)) = unroll (memD mem (sem (prog_optimise prog) st))
+). destruct (memD mem (sem (prog_optimise prog) st)); eauto. rewrite H. clear H.
 
-rewrite H. simpl. admit.
+(*unroll*)
+simpl.
+
+
+(*unfold stepD*)
+unfold stepD.
+unfold CFG.fetch. destruct st. destruct p. destruct p.
+unfold CFG.find_function.
 
 
 
 
 
+destruct prog. simpl.
+destruct m_definitions. simpl.
+(*no instruction*)
+  -constructor. constructor.
+  -destruct d. simpl.
+unfold find_defn. 
+unfold cfg_opt. simpl.
+destruct df_instrs. simpl in *.
+unfold alter_blocks. simpl.
+unfold optimise.
+unfold map.
+unfold AstLib.ident_of.
+unfold AstLib.ident_of_definition.
+simpl.
+destruct (AstLib.ident_of df_prototype == ID_Global fn); simpl.
+    +simpl. destruct blks.
+{
+simpl. constructor. constructor.
+}
+{
+simpl.
+unfold terminator_check. simpl. destruct b.
+simpl. 
 
 
 
-  +(*full blks*) admit.
-Admitted.
+(*NOT SURE*)
+
+
+
+destruct blk_term. simpl.
+induction t.
+    -simpl. admit.
+    -simpl. admit.
+    -simpl. admit.
+    -simpl. admit.
+    -simpl. admit.
+    -simpl. admit.
+    -simpl. admit.
+    -simpl. admit.
+}
+  +unfold not in n.
+unfold AstLib.ident_of.
+unfold AstLib.ident_of_declaration.
+unfold dc_name.
+(*UNFOLD IN TWO*)
